\documentclass[a4paper,10pt]{article}
\usepackage[utf8x]{inputenc}
\usepackage[hmargin=30mm, vmargin=15mm]{geometry}
\usepackage{CalcStyleV8}
\usepackage[linkcolor=black, colorlinks=true, pagebackref=true]{hyperref}

%opening
\title{1FC3 Theorem List}
\author{JK}

\newenvironment{theoremlist}{
\begin{description}
  \setlength{\itemsep}{1.5pt}
  \setlength{\parskip}{0pt}
  \setlength{\parsep}{0pt}
}{\end{description}}

\DeclareMathSymbol{\mlq}{\mathord}{operators}{``}
\DeclareMathSymbol{\mrq}{\mathord}{operators}{`'}


\begin{document}

\maketitle
\thispagestyle{empty}

\newpage
\tableofcontents %put toc in
\thispagestyle{empty}

\cleardoublepage %start new page

\setcounter{page}{1} %reset the page counter

\section{Equivalence}

\begin{theoremlist}
\item[(3.1) Axiom, Associativity of $\equiv$:] 					$ ((p \equiv q) \equiv r) \equiv (p \equiv (q \equiv r)) $
\item[(3.2) Axiom, Symmetry of $\equiv$:] 					$ p \equiv q \equiv q \equiv p $
\item[(3.3) Axiom, Identity of $\equiv$:] 					$ \true \equiv q \equiv q $
\item[(3.4)] 									$ \true $
\item[(3.5) Reflexivity of $ \equiv$:] 						$ p \equiv p $
\item[(3.7) Metatheorem:] 							Any two theorems are equivalent.
\end{theoremlist}


\section{Negation}

\begin{theoremlist}
\item[(3.8) Axiom, Definition of $\false$:] 					$ \false \equiv \lnot \true $
\item[(3.9) Axiom, Distributivity of $\lnot$ over $\equiv$:]			$ \lnot (p \equiv q) \equiv (\lnot p \equiv q) $
\item[(3.10) Axiom, Definition of $\nequiv$:]					$ (p \nequiv q) \equiv \lnot (p \equiv q) $
\item[(3.11)] 									$ \lnot p \equiv q \equiv p \equiv \lnot q $
\item[(3.12) Double negation:]							$ \lnot\lnot p \equiv p $
\item[(3.13) Negation of $\false$:]						$ \lnot \false \equiv \true $
\item[(3.14)]									$ (p \nequiv q) \equiv \lnot p \equiv q $
\item[(3.15)] 									$ \lnot p \equiv p \equiv \false $
\item[(3.16) Symmetry of $\nequiv$:]						$ (p \nequiv q) \equiv (q \nequiv p) $
\item[(3.17) Associativity of $\nequiv$:]					$ ((p \nequiv q) \nequiv r) \equiv (p \nequiv (q \nequiv r)) $
\item[(3.18) Mutual associativity:]						$ ((p \nequiv q) \equiv r) \equiv (p \nequiv (q \equiv r)) $
\item[(3.19) Mutual interchangeability:]					$ p \nequiv q \equiv r \equiv p \equiv q \nequiv r $
\end{theoremlist}



\section{Disjunction}

\begin{theoremlist}
\item[(3.24) Axiom, Symmetry of $\lor$:] 					$ p \lor q \equiv q \lor p $
\item[(3.25) Axiom, Associativity of $\lor$:]					$ (p \lor q) \lor r \equiv p \lor (q \lor r) $ 
\item[(3.26) Axiom, Idempotency of $\lor$:]					$ p \lor p \equiv p $
\item[(3.27) Axiom, Distributivity of $\lor$ over $\equiv$:]			$ p \lor (q \equiv r) \equiv p \lor q \equiv p \lor r $
\item[(3.28) Axiom, Excluded Middle:]						$ p \lor \lnot p $
\item[(3.29) Zero of $\lor$:]							$ p \lor \true \equiv true $
\item[(3.30) Identity of $\lor$:]						$ p \lor \false \equiv p $
\item[(3.31) Distributivity of $\lor$ over $\lor$:]				$ p \lor (q \lor r) \equiv (p \lor q) \lor (p \lor r) $
\item[(3.32)]									$ p \lor q \equiv p \lor \lnot q \equiv p $
\end{theoremlist}


\section{Conjunction}

\begin{theoremlist}
\item[(3.35) Axiom, Golden rule:]						$ p \land q \equiv p \equiv q \equiv p \lor q $
\item[(3.36) Symmetry of $\land$:]						$ p \land q \equiv q \land p $
\item[(3.37) Associativity of $\land$:]						$ (p \land q) \land r \equiv p \land (q \land r) $
\item[(3.38) Idempotency of $\land$:]						$ p \land p \equiv p $
\item[(3.39) Identity of $\land$:]						$ p \land \true \equiv p $
\item[(3.40) Zero of $\land$:]							$ p \land \false \equiv \false  $
\item[(3.41) Distributivity of $\land$ over $\land$:]				$ p \land (q \land r) \equiv (p \land q) \land (p \land r) $
\item[(3.42) Contradiction:]							$ p \land \lnot p \equiv \false $
\item[(3.43) Absorption:]						
  \begin{theoremlist}
  \item %intentionally blank
  \item[(a)]									$ p \land (p \lor q) \equiv p $
  \item[(b)] 									$ p \lor (p \land q) \equiv p $
  \end{theoremlist}                  						                               	              
\item[(3.44) Absorption:]
  \begin{theoremlist}
  \item %intentionally blank
  \item[(a)]									$ p \land (\lnot p \lor q) \equiv p \land q $
  \item[(b)] 									$ p \lor (\lnot p \land q) \equiv p \lor q $
  \end{theoremlist}      
\item[(3.45) Distributivity of $\lor$ over $\land$:]				$ p \lor (q \land r) \equiv (p \lor q) \land (p \lor r) $
\item[(3.45) Distributivity of $\land$ over $\lor$:]				$ p \land (q \lor r) \equiv (p \land q) \lor (p \land r) $
\item[(3.47) De Morgan:]
  \begin{theoremlist}
  \item %intentionally blank
  \item										$ \lnot(p \land q) \equiv \lnot p \lor \lnot q $
  \item 									$ \lnot(p \lor q) \equiv \lnot p \land \lnot q $
  \end{theoremlist}      
\item[(3.48):]									$ p \land q \equiv p \land \lnot q \equiv \lnot p $
\item[(3.49):]									$ p \land (q \equiv r) \equiv p \land q \equiv p \land r \equiv p $
\item[(3.50):]									$ p \land (q \equiv p) \equiv p \land q	$
\item[(3.51) Replacement:]							$ (p \equiv q ) \land (r \equiv p) \equiv (p \equiv q) \land (r \equiv q) $
\item[(3.52) Definition of $\equiv$:]						$ p \equiv q \equiv (p \land q) \lor (\lnot p \land \lnot q) $
\item[(3.53) Definition of $\nequiv$ (Exclusive or):]				$ p \nequiv q \equiv (\lnot p \land q) \lor (p \land \lnot q) $
\end{theoremlist}


\section{Implication}

\begin{theoremlist}
\item[(3.57) Axiom, Definition of Implication:]					$ p \implies q \equiv p \lor q \equiv q $
\item[(3.58) Axiom, Consequence:]						$ p \follows q \equiv q \implies p $
\item[(3.59) (Alternative) Definition of Implication:]				$ p\implies q \equiv \lnot p \lor q $
\item[(3.60) (Dual) Definition of Implication:]					$ p \implies q \equiv p \land q \equiv p $
\item[(3.61) Contrapositive:]							$ p \implies q \equiv \lnot q \implies \lnot p $

\item[Ex. 3.45]									$ p \implies q \equiv \lnot p \lor \lnot q \equiv \lnot p $
\item[Ex. 3.46]									$ p \implies q \equiv \lnot p \land \lnot q \equiv \lnot q $
\item[(3.62:]									$ p \implies (q \equiv r) \equiv p \land q \equiv p \land r $
\item[(3.63) Distributivity of $\implies$ over $\equiv$:]			$ p \implies (q \equiv r) \equiv p \implies q \equiv p \implies r $
\item[(3.64) Self-distributivity of $\implies$:]				$ p \implies (q \implies r) \equiv (p \implies q) \implies (p \implies r)$
\item[(3.65) Shunting:]								$ p \land q \implies r \equiv p \implies (q \implies r) $
\item[(3.66)]									$ p \land (p \implies q) \equiv p \land q $
\item[(3.67)]									$ p \land (q \implies p) \equiv p $
\item[(3.68)]									$ p \lor (p \implies q) \equiv \true $
\item[(3.69)]									$ p \lor (q \implies p) \equiv q \implies p $
\item[(3.70)]									$ p \lor q \implies p \land q \equiv p \equiv q$
\item[(3.71) Reflexivity of $\implies$:]					$ p \implies p \equiv \true $
\item[(3.72) Right zero of $\implies$:]						$ p \implies \true \equiv \true $
\item[(3.73) Left identity of $\implies$:]					$ \true \implies p \equiv p $
\item[(3.74)]									$ p \implies \false \equiv \lnot p $
\item[(3.75)]									$ \false \implies p \equiv true $
\item[(3.76) Weakening/strengthening:]
  \begin{theoremlist}
  \item %intentionally blank
  \item[(a)]									$ p \implies p \lor q $
  \item[(b)] 									$ p \land q \implies p $
  \item[(c)] 									$ p \land q \implies p \lor q $
  \item[(d)] 									$ p \lor (q \land r) \implies p \lor q $
  \item[(e)] 									$ p \land q \implies p \land (p \lor r) $
  \end{theoremlist} 
\item[(3.77) Modus ponens:]							$ p \land (p \implies q) \implies q $
\item[(3.78) Case analysis:]							$ (p \implies r) \land (q \implies r) \equiv (p \lor q \implies r) $
\item[(3.79) Case analysis:]							$ (p \implies r) \land (\lnot p \implies r) \equiv r $							
\item[(3.80) Mutual implication:]						$ (p \implies q) \land (q \implies p) \equiv p \equiv q $
\item[(3.80b) Reflexivity wrt. Equivalence:]					$ (p \equiv q) \implies (p \implies q) $
\item[(3.81) Antisymmetry:]							$ (p \implies q) \land (q \implies p) \implies p \equiv q $
\item[(3.82) Transitivity:]							
  \begin{theoremlist}
  \item %intentionally blank
  \item[(a)]									$ (p \implies q) \land (q \implies r) \implies (p \implies r) $
  \item[(b)] 									$ (p \equiv q) \land (q \implies r) \implies (p \implies r) $
  \item[(c)] 									$ (p \implies q) \land (q \equiv r) \implies (p \implies r) $
  \end{theoremlist}
\item[Ex. 6.3.A]								$ p \implies (q \land r) \equiv (p \implies q) \land (p \implies r) $
\item[Ex. 6.3.B]								$ (p \land q) \lor (\lnot p \land r) \equiv (p \implies q) \land (\lnot p \implies r) $
\item[Ex. 6.3.C]								$ (p \land q) \lor (\lnot p \land r) \equiv (\lnot p \lor r) \land (p \lor r) $
\item[Ex. 6.3.D]								$ \lnot p \lor (p \implies q) \equiv p \implies q $
\item[Ex. 6.3.E]								$ p \lor (\lnot p \implies q) \equiv \lnot p \implies q $
\item[(4.1)]									$ p \implies (q \implies p) $
\item[(4.2) Monotonicity of $\lor$:]						$ (p \implies q) \implies (p \lor r \implies q \lor r) $
\item[(4.3) Monotonicity of $\land$:]						$ (p \implies q) \implies p \land r \implies q \land r $
\item[(4.4) (Extended) Deduction Theorem:]					Suppose adding $P_1 ,\ldots, P_n$ as axioms to
										propositional logic $\mathbf{E}$, with the variables of the $Pi$ considered to be constants,
										allows $Q$ to be proved.
										Then $P_1 \land \ldots \land P_n \implies Q$ is a theorem.
\item[(4.6)]									$ (p \lor q \lor r) \land (p \implies s) \land (q \implies s) \land (r \implies s) \implies s $


\end{theoremlist}


\section{Substitution (Leibniz as an axiom)}

\begin{theoremlist}
\item[(3.84a)]									$ (e = f) \land E[z \becomes e] \equiv (e = f) \land E[z \becomes f] $
\item[(3.84b)]									$ (e = f) \implies E[z \becomes e] \equiv (e = f) \implies E[z \becomes f] $
\item[(3.84c)]									$ q \land (e = f) \implies E[z \becomes e] \equiv q \land (e = f) \implies E[z \becomes f] $
\item[(3.85a) Replace by $\true$:]						$ p \implies E[z \becomes p] \equiv p \implies E[z \becomes \true] $
\item[(3.85b) Replace by $\true$:]						$ q \land p \implies E[z \becomes p] \equiv \land p \implies E[z \becomes \true] $
\item[(3.86a) Replace by $\false$:]						$ E[z \becomes p] \implies p \equiv E[z \becomes \false] \implies p $
\item[(3.86b) Replace by $\false$:]						$ E[z \becomes p] \implies p \lor q \equiv E[z \becomes \false] \implies p \lor q $
\item[(3.87) Replace by $\true$:]						$ p \land E[z \becomes p] \equiv p \land E[z \becomes \true] $
\item[(3.88) Replace by $\false$:]						$ p \lor E[z \becomes p] \equiv p \lor E[z \becomes \false] $
\item[(3.89) Shannon:]								$ E[z \becomes p] \equiv (p \land E[z \becomes \true]) \lor (\lnot p \land E[z \becomes \false]) $
\item[(4.5) Metatheorem, Case analysis (Shannon):]				$\break$ If $E[z \becomes \true]$ and $E[z \becomes \false]$ are theorems, then so is $E[z \becomes p] $ 
\end{theoremlist}


\section{Quantification}
\subsection{General laws of quantification}

\begin{theoremlist}
\item[(8.11) Substitution:]							Provided $ \lnot occurs(\mlq y \mrq,\mlq x,F \mrq) $,\newline
										$ (\star x \with R \spot P)[x \becomes F] = (\star x \with R[x \becomes F] \spot P[x \becomes F] $
										
\item[(8.13) Axiom, Empty range (where $u$ is the identity of $\star$):]	$ (\star x \with \false \spot P) = u $

\item[(8.14) Axiom, One-point rule:]						Provided $ \lnot occurs(\mlq x \mrq, \mlq E \mrq) $,\newline
										$ (\star x \with x = E \spot P) = P[x \becomes E] $

\item[(8.15) Axiom, (Quantification) Distributivity:]				Provided each quantification is defined,\newline
										$ (\star x \with R \spot P) \star (\star x \with R \spot Q) = (\star x \with R \spot P \star Q) $

\item[(8.16) Axiom, Range split:]						Provided $ R \land S = \false $ and each quantification is defined,\newline
										$ (\star x \with R \lor S \spot P) = (\star x \with R \spot P) \star (\star x \with S \spot P) $

\item[(8.17) Axiom, Range split:]						Provided each quantification is defined,\newline
										$ (\star x \with R \lor S \spot P) \star (\star x \with R \land S \spot P) = (\star x \with R \spot P) \star (\star x \with S \spot P) $

\item[(8.18) Range split for idempotent $\star$:]				Provided each quantification is defined,\newline
										$ (\star x \with R \lor S \spot P) = (\star x \with R \spot P) \star (\star x \with S \spot P) $

\item[(8.19) Axiom, Interchange of dummies:]					Provided $ \lnot occurs (\mlq y \mrq, \mlq R \mlq)$ and $ \lnot occurs (\mlq x \mrq, \mlq S \mlq)$, and each quantification is defined,\newline 
										$ (\star x \with R \spot (\star y \with S \spot P)) = (\star y \with R \spot (\star x \with S \spot P)) $

\item[(8.20) Axiom, Nesting:]							Provided $ \lnot occurs (\mlq y \mrq, \mlq R \mlq)$,\newline	
										$ (\star x,y \with R \land S \spot P) = (\star x \with R \spot (\star y \with S \spot P)) $

\item[(8.20a) Axiom, Dummy list permutation:]					$ (\star x,y \with R \spot P) = (\star y,x \with R \spot P) $

\item[(8.21) Axiom, Dummy renaming ($\alpha$ conversion):]			Provided $ \lnot occurs (\mlq y \mrq, \mlq R,P \mlq)$,\newline
										$ (\star x \with R \spot P) = (\star y \with R[x \becomes y] \spot P[x \becomes y]) $

\item[(8.22) Change of dummy:]							Provided $ f $ has an inverse and $ \lnot occurs (\mlq y \mrq, \mlq x,R,P \mlq)$,\newline
										$ (\star x \with R \spot P) = (\star y \with R[x \becomes f.y] \spot P[x \becomes f.y]) $

\item[(8.23) Theorem Split off term:]						For $n:\NN$ and dummies $i:\NN$,\newline			
										$ (\star x \with 0 \leq i < n + 1 \spot P) = (\star x \with 0 \leq i < n \spot P) \star P[i \becomes n] $
										\newline
										$ (\star x \with 0 \leq i < n + 1 \spot P) = P[i \becomes 0] \star (\star i \with 0 < i < n + 1 \spot P) $
\end{theoremlist}


\subsection{Universal Quantification}

\begin{theoremlist}
\item[(9.2) Axiom, Trading:]							$ (\forall x \with R \spot P) \equiv (\forall x \withspot R \implies P) $
\item[(9.3) Trading:]
  \begin{theoremlist}
  \item %intentionally blank
  \item[(a)]									$ (\forall x \with R \spot P) \equiv (\forall x \withspot \lnot R \lor P) $
  \item[(b)] 									$ (\forall x \with R \spot P) \equiv (\forall x \withspot R \land P \equiv R) $
  \item[(c)] 									$ (\forall x \with R \spot P) \equiv (\forall x \withspot R \lor P \equiv P) $
  \end{theoremlist}
\item[(9.4) Trading:]
  \begin{theoremlist}
  \item %intentionally blank
  \item[(a)]									$ (\forall x \with Q \land R \spot P) \equiv (\forall x \with Q \spot R \implies P) $
  \item[(b)] 									$ (\forall x \with Q \land R \spot P) \equiv (\forall x \with Q \spot \lnot R \lor P) $
  \item[(c)] 									$ (\forall x \with Q \land R \spot P) \equiv (\forall x \with Q \spot R \land P \equiv R) $
  \item[(d)] 									$ (\forall x \with Q \land R \spot P) \equiv (\forall x \with Q \spot R \lor P \equiv P) $
  \end{theoremlist}
\item[(9.4.1) Universal double trading:]					$ (\forall x \with R \spot P) \equiv (\forall x \with P \spot R) $

\item[(9.5) Axiom, Distributivity of $\lor$ over $\forall$:]			Provided $ \lnot occurs (\mlq x \mrq, \mlq P \mlq)$,\newline
										$ P \lor (\forall x \with R \spot Q) \equiv (\forall x \with R \spot P \lor Q) $

\item[(9.6)]									Provided $ \lnot occurs (\mlq x \mrq, \mlq P \mlq)$, 
										$ (\forall x \with R \spot P) \equiv P (\forall x \withspot \lnot R) $

\item[(9.7) Axiom, Distributivity of $\land$ over $\forall$:]			Provided $ \lnot occurs (\mlq x \mrq, \mlq P \mlq)$,\newline
										$ \lnot(\forall \withspot \lnot R) \implies ((\forall x \with R \spot P \land Q) \equiv P \land (\forall x \with R \spot Q)) $

\item[(9.8]									$ (\forall x \with R \spot \true) \equiv \true $
\item[(9.9)]									$ (\forall x \with R \spot P \equiv Q) \implies ((\forall x \with R \spot P) \equiv (\forall x \with R \spot Q)) $
\item[(9.10) Range weakening/strengthening:]					$ (\forall x \with R \lor Q \spot P) \implies (\forall x \with R \spot P) $   
\item[(9.11) Body weakening/strengthening:]					$ (\forall x \with R \spot P \land Q) \implies (\forall x \with R \spot P) $   
\item[(9.12) Monotonicity of $\forall$:]					$ (\forall x \with R \spot Q \implies P) \implies ((\forall x \with R \spot Q) \implies (\forall x \with R \spot P)) $
\item[(9.12a) Range-antitonicity of $\forall$:]					$ (\forall x \withspot Q \implies R) \implies ((\forall x \with R \spot P) \implies (\forall x \with Q \spot P)) $
\item[(9.13) Instantiation:]							$ (\forall x \withspot P) \implies P[x \becomes E] $   
\item[(9.16) Metatheorem:]							$ P $ is a theorem iff $ (\forall x \withspot P) $ is a theorem. 


\end{theoremlist}


\subsection{Existential Quantification}

\begin{theoremlist}
\item[(9.17) Axiom, Generalized De Morgan:]					$ (\exists x \with R \spot P) \equiv \lnot (\forall x \with R \spot \lnot P) $
\item[(9.18) Generalized De Morgan:]
  \begin{theoremlist}
  \item %intentionally blank
  \item[(a)]									$ \lnot (\exists x \with R \spot \lnot P) \equiv (\forall x \with R \spot P) $
  \item[(b)] 									$ \lnot (\exists x \with R \spot P) \equiv (\forall x \with R \spot \lnot P) $
  \item[(c)] 									$ (\exists x \with R \spot \lnot P) \equiv \lnot(\forall x \with R \spot P) $
  \end{theoremlist}
\item[(9.19) Trading for $\exists$:]						$ (\exists x \with R \spot P) \equiv (\exists x \withspot R \land P) $
\item[(9.20) Trading for $\exists$:]						$ (\exists x \with Q \land R \spot P) \equiv (\exists x \with Q \spot R \land P) $
\item[(9.20.1) Existential double trading:]					$ (\exists x \with R \spot P) \equiv (\exists x \with P \spot R) $
\item[(9.20.2)]									$ (\exists x \withspot R) \implies ((\forall x \with R \spot P) \implies (\exists x \with R \spot P)) $

\item[(9.21) Distributivity of $\land$ over $\exists$:]				Provided $ \lnot occurs (\mlq x \mrq, \mlq P \mlq)$,\newline
										$ P \land (\exists x \with R \spot Q) \equiv (\exists x \with R \spot P \land Q) $

\item[(9.22)]									Provided $ \lnot occurs (\mlq x \mrq, \mlq P \mlq)$,
										$ (\exists x \with R \spot P) \equiv P \land (\exists x \withspot R) $

\item[(9.23) Distributivity of $\lor$ over $\exists$:]				Provided $ \lnot occurs (\mlq x \mrq, \mlq P \mlq)$,\newline
										$ (\exists x \withspot R) \implies ((\exists x \with R \spot P \lor Q) \equiv P \lor (\exists x \with R \spot Q)) $

\item[(9.24)]									$ (\exists x \with R \spot \false) \equiv \false $
\item[(9.25) Range weakening/strengthening:]					$ (\exists x \with R \spot P) \implies (\exists x \with Q \lor R \spot P) $
\item[(9.26) Body weakening/strengthening:]					$ (\exists x \with R \spot P) \implies (\exists x \with R \spot P \lor Q) $
\item[(9.27) (Body) Monotonicity of $\exists$:]					$ (\exists x \with R \spot Q \implies P) \implies ((\exists x \with R \spot Q) \implies (\exists x \with R \spot P)) $
\item[(9.27) Range-Monotonicity of $\exists$:]					$ (\exists x \withspot Q \implies R) \implies ((\exists x \with Q \spot P) \implies (\exists x \with R \spot P)) $
\item[(9.28) $\exists$ Introduction:]						$ P[x \becomes p] \implies (\exists x \withspot P) $

\item[(9.29) Interchange of quantifications:]					Provided $ \lnot occurs (\mlq y \mrq, \mlq R \mlq) \land \lnot occurs (\mlq x \mrq, \mlq Q \mlq)$,\newline
										$ (\exists x \with R \spot (\forall y \with Q \spot P)) \implies (\forall y \with Q \spot (\exists x \with R \spot P)) $

\item[(9.30) Metatheorem Witness:]						If $ \lnot occurs (\mlq \hat{x} \mrq, \mlq P,Q,R \mlq)$, then:\newline
										$ (\exists x \with R \spot P) \implies Q $ is a theorem iff $ (R \land P)[x \becomes \hat{x}] \implies Q $ is a theorem.

\item[(9.30v) Metatheorem Witness (variant):]					If $ \lnot occurs (\mlq x \mrq, \mlq Q \mlq)$, then:\newline
										$ (\exists x \with R \spot P) \implies Q $ is a theorem iff $ (R \land P) \implies Q $ is a theorem.

\end{theoremlist}

\section{Sets}
\subsection{General set theorems}

\begin{theoremlist}
\item[(11.2)]									$  $
\item[(11.3)]									$  $
\item[(11.4)]									$  $
\item[(11.4e)]									$  $
\item[(11.5)]									$  $
\item[(11.6)]									$  $
\item[(11.7)]									$  $
\item[(11.8)]									$  $
\item[(11.9)]									$  $
\item[(11.10)]									$  $
\item[(11.11)]									$  $
\end{theoremlist}

\subsection{Operations on sets}

\begin{theoremlist}
\item[(11.12)]									$  $
\item[(11.13)]									$  $
\item[(11.14)]									$  $
\item[(11.15)]									$  $
\item[(11.16)]									$  $
\item[(11.17)]									$  $
\item[(11.18)]									$  $
\item[(11.19)]									$  $
\item[(11.20)]									$  $
\item[(11.21)]									$  $
\item[(11.22)]									$  $
\item[(11.24)]									$  $
\item[(11.25)]									$  $
\end{theoremlist}

\subsection{Basic properties of union}
\begin{theoremlist}
\item[(11.26)]									$  $
\item[(11.27)]									$  $
\item[(11.28)]									$  $
\item[(11.29)]									$  $
\item[(11.30)]									$  $
\item[(11.31)]									$  $
\item[(11.32)]									$  $
\end{theoremlist}

\subsection{Basic properties of intersection}
\begin{theoremlist}
\item[(11.33)]									$  $
\item[(11.34)]									$  $
\item[(11.35)]									$  $
\item[(11.36)]									$  $
\item[(11.37)]									$  $
\item[(11.38)]									$  $
\item[(11.39)]									$  $
\end{theoremlist}

\subsection{Properties of combinations of union and intersection}
\begin{theoremlist}
\item[(11.40)]									$  $
\item[(11.41)]									$  $
\item[(11.42)]									$  $
\item[(11.43)]									$  $
\item[(11.44)]									$  $
\item[(11.45)]									$  $
\item[(11.46)]									$  $
\item[(11.47)]									$  $
\item[(11.48)]									$  $
\end{theoremlist}

\subsection{Properties of set difference}
\begin{theoremlist}
\item[(11.49)]									$  $
\item[(11.50)]									$  $
\item[(11.51)]									$  $
\item[(11.52)]									$  $
\item[(11.53)]									$  $
\item[(11.54)]									$  $
\item[(11.55)]									$  $	
\end{theoremlist}

\subsection{Implication versus subset}
\begin{theoremlist}
\item[(11.56)]									$  $
\end{theoremlist}

\subsection{Subsets}
\begin{theoremlist}
\item[(11.57)]									$  $
\item[(11.58)]									$  $
\item[(11.59)]									$  $
\item[(11.60)]									$  $
\item[(11.61)]									$  $
\item[(11.62)]									$  $
\item[(11.63)]									$  $
\item[(11.64)]									$  $
\item[(11.65)]									$  $
\item[(11.66)]									$  $
\item[(11.67)]									$  $
\item[(11.68)]									$  $
\item[(11.69)]									$  $
\item[(11.70)]									$  $
\end{theoremlist}

\subsection{Powersets}
\begin{theoremlist}
\item[(11.71)]									$  $
\item[(11.72)]									$  $
\item[(11.73)]									$  $
\end{theoremlist}


\end{document}
